theories/examples/compression/buffers_adequacy.v
@@ -1,0 +1,65 @@
+From iris.proofmode Require Import coq_tactics reduction spec_patterns.
+From iris.proofmode Require Export tactics.
+From iris.prelude Require Import options.
+From melocoton Require Import named_props.
+From melocoton.linking Require Import lang weakestpre.
+From melocoton.lang_to_mlang Require Import lang weakestpre.
+From melocoton.interop Require Import basics basics_resources wp_simulation.
+From melocoton.interop Require Import lang weakestpre update_laws wp_utils prims_proto.
+From melocoton.language Require Import weakestpre progenv.
+From melocoton.c_interop Require Import rules notation.
+From melocoton.c_lang Require Import mlang_instantiation lang_instantiation.
+From melocoton.ml_lang Require primitive_laws proofmode.
+From melocoton.c_lang Require Import notation proofmode derived_laws.
+From melocoton.ml_lang Require Import notation lang_instantiation.
+From melocoton.combined Require Import adequacy.
+From melocoton.examples.compression Require Import buffers_proofs buffers_specs buffers_client.
+
+
+Section FixpointSpec.
+  Context `{SI:indexT}.
+  Context `{!heapG_C Σ, !heapG_ML Σ, !invG Σ, !primitive_laws.heapG_ML Σ, !wrapperG Σ}.
+
+  Definition buf_library_spec_ML E := fixpoint (buf_library_spec_ML_pre E).
+  Lemma buf_library_spec_ML_unfold E s vv Φ :
+   (buf_library_spec_ML E s vv Φ ⊣⊢ buf_library_spec_ML_pre E (buf_library_spec_ML E) s vv Φ)%I.
+  Proof.
+    exact (fixpoint_unfold (buf_library_spec_ML_pre E) s vv Φ).
+  Qed.
+  Lemma buf_library_spec_ML_sim E:
+   (buf_library_spec_ML E ⊑ buf_library_spec_ML_pre E (buf_library_spec_ML E))%I.
+  Proof.
+    iIntros (s vv Φ) "H". by iApply buf_library_spec_ML_unfold.
+  Qed.
+
+  Lemma ML_client_applied_spec_fix E:
+    {{{ True }}}
+      ML_client_applied_code @ ML_client_env E (buf_library_spec_ML E) ; E
+    {{{ x, RET #x ; ⌜x=1%Z⌝ }}}.
+  Proof.
+    apply ML_client_applied_spec.
+  Qed.
+
+End FixpointSpec.
+
+Local Existing Instance ordinals.ordI.
+
+Definition fullprog : mlang_prog combined_lang :=
+  combined_prog ML_client_applied_code buf_lib_prog_total.
+
+Lemma buffers_adequate :
+  umrel.trace (mlanguage.prim_step fullprog) (LkCall "main" [], adequacy.σ_init)
+    (λ '(e, σ), mlanguage.to_val e = Some (code_int 1)).
+Proof.
+  eapply umrel_upclosed.
+  { eapply combined_adequacy_trace. intros Σ Hffi E. split_and!.
+    3: apply ML_client_applied_spec_fix.
+    3: { rewrite wrap_proto_mono. 1: apply buffer_library_correct.
+         apply buf_library_spec_ML_pre_mono, buf_library_spec_ML_sim. }
+    { iIntros (? Hn ?) "(% & H)". unfold prim_names in H.
+      rewrite !dom_insert dom_empty /= in H.
+      iDestruct "H" as "[[[[H|H]|H]|H]|H]".
+      all: iNamed "H"; exfalso; cbn in H; set_solver. }
+    { set_solver. } }
+  { by intros [? ?] (? & ? & ->). }
+Qed.
