theories/examples/compression/buffers_client.v
@@ -1,0 +1,190 @@
+From iris.proofmode Require Import coq_tactics reduction spec_patterns.
+From iris.proofmode Require Export tactics.
+From iris.prelude Require Import options.
+From melocoton Require Import named_props.
+From melocoton.interop Require Import basics basics_resources basics_constructions.
+From melocoton.interop Require Import lang weakestpre.
+From melocoton.language Require Import weakestpre progenv.
+From melocoton.ml_lang Require Import notation lang_instantiation.
+From melocoton.ml_lang Require primitive_laws proofmode.
+From melocoton.c_interface Require Import defs notation resources.
+From melocoton.examples.compression Require Import buffers_specs buffers_laws compression_defs.
+
+
+Section MLclient.
+
+  Context `{SI:indexT}.
+  Context `{!heapG_C Σ, !heapG_ML Σ, !invG Σ, !primitive_laws.heapG_ML Σ, !wrapperG Σ}.
+  Import melocoton.ml_lang.notation melocoton.ml_lang.lang_instantiation
+         melocoton.ml_lang.primitive_laws melocoton.ml_lang.proofmode.
+
+  Context (E : coPset).
+  Context (Ψ : (protocol ML_lang.val Σ)).
+
+  Definition ML_client_env : prog_environ ML_lang Σ := {|
+    penv_prog  := ∅ ;
+    penv_proto := buf_library_spec_ML_pre E Ψ |}.
+
+  Definition ML_client_code : MLval := 
+    λ: "vbuf",
+      let: "len"  := Length "vbuf" in
+      let: "inp"  := extern: buf_alloc_name with ("len") in
+      let: "outp" := extern: buf_alloc_name with (extern: wrap_max_len_name with ("len")) in
+      let: <>     := extern: buf_upd_name with (#0, "len" - #1, λ: "i", LoadN "vbuf" "i", "inp") in
+      let: <>     := extern: wrap_compress_name with ("inp", "outp") in
+      let: "shrn" := ! (Fst "outp") < ! (Fst "inp") in
+      let: <>     := extern: buf_free_name with ("inp") in
+      let: <>     := extern: buf_free_name with ("outp") in
+      "shrn".
+
+  Definition is_compressible (zz : buffer) :=
+    let P := length (compress_buffer zz) < length zz
+    in decide P.
+
+
+
+  Lemma ML_client_spec ℓ dq (zz : buffer) :
+    0 < length zz →
+    {{{ ℓ ↦∗{dq} map (λ (x:Z), #x) zz }}}
+      ML_client_code #ℓ @ ML_client_env ; E
+    {{{ RET #(if is_compressible zz then true else false); ℓ ↦∗{dq} map (λ (x:Z), #x) zz }}}.
+  Proof.
+    iIntros (Hlen Φ) "Hℓ Cont".
+    unfold ML_client_code, ML_client_env. wp_pures.
+    wp_apply (wp_length with "Hℓ"); iIntros "Hℓ". wp_pures.
+
+    wp_extern. iModIntro. cbn. do 4 iLeft. rewrite !map_length.
+    iExists (length zz). iSplit; first (iPureIntro; lia).
+    iSplit; first done. iSplit; first done.
+    iNext. iIntros (vin ℓinbuf) "Hinbuf _". wp_finish.
+    wp_pures.
+
+    wp_extern. iModIntro. iRight.
+    iExists _.
+    iSplit; first done. iSplit; first done.
+    iNext. wp_pures.
+
+    wp_extern. iModIntro. do 4 iLeft.
+    iExists _. iSplit.
+    2: iSplit; first done. 2: iSplit; first done.
+    1: iPureIntro; lia.
+    iNext. iIntros (vout ℓoutbuf) "Houtbuf _". wp_finish.
+    wp_pures.
+
+    wp_extern. iModIntro. do 3 iLeft; iRight.
+
+    pose (λ (idx:Z) (used:nat) (b : list (option Z)), 
+        ∃ zpre zopost zzpost, ⌜b = map Some zpre ++ zopost⌝ ∗ ⌜length zopost = length zzpost⌝ ∗ 
+        ⌜zz = zpre ++ zzpost⌝ ∗ ⌜Z.of_nat used = idx⌝ ∗ ⌜Z.of_nat (length zpre) = idx⌝ : iProp Σ)%I as Hbufatidx.
+
+    pose (λ (idx:Z), isBufferRecordML vin ℓinbuf (Hbufatidx idx) (length zz) ∗ (ℓ ↦∗{dq} map (λ x : Z, #x) zz))%I as Ψ'.
+    pose (λ (idx:Z), (ℓ ↦∗{dq} map (λ x : Z, #x) zz))%I as Ψframe.
+    pose (λ (idx:Z) (z:Z), ∃ n, ⌜Z.of_nat n = idx⌝ ∗ ⌜zz !! n = Some z⌝ : iProp Σ)%I as Φz.
+    iExists Ψ', Ψframe, Φz, _, _, _, _. iExists Hbufatidx, _, _, _, _. unfold named.
+    iSplit; first done.
+    iSplit; first done.
+    iSplit; first done.
+    iSplit; first (iPureIntro; lia).
+    iPoseProof (isBufferRecordML_ext with "[] Hinbuf") as "Hinbuf".
+    2: iFrame "Hinbuf Hℓ".
+    { iIntros (z lst) "(->&->)". iExists nil, _, _. cbn. repeat (iSplit; first done). iSplit. 2: iSplit; first done. 2: done.
+      rewrite replicate_length. iPureIntro; lia. }
+    iSplit; first (iPureIntro; lia).
+    iSplit; last iSplit; last iSplitR.
+    all: unfold Ψframe, Φz, Ψ'; rewrite !Nat2Z.id.
+    { iIntros "!> %z %vnew %Hz0 %Hzlen Hframe (%n&<-&%Hz) HBuffer".
+      iModIntro. iFrame "Hframe". iApply (isBufferRecordML_ext with "[] HBuffer").
+      iIntros (z lst). unfold buf_alloc1_spec, Hbufatidx.
+      iIntros "(%bold&%capold&->&->&%zpre&%zopost&%zzpost&->&%Hzzlen&->&%Heq1&%Heq2)".
+      apply Nat2Z.inj' in Heq2. subst n.
+      destruct zzpost as [|vnew' zzpost].
+      { exfalso. rewrite app_nil_r in Hz. apply lookup_lt_Some in Hz. lia. }
+      rewrite lookup_app_r in Hz; last lia. 
+      rewrite Nat.sub_diag in Hz. cbn in Hz. simplify_eq.
+      destruct zopost as [|zoh zopost]; first done.
+      iExists (zpre ++ [vnew]), zopost, zzpost.
+      rewrite !Nat2Z.id !map_app -!app_assoc /=.
+      iPureIntro; split_and!; try done.
+      - replace (length zpre) with (length (map Some zpre) + 0) by (rewrite map_length; lia).
+        rewrite insert_app_r. done.
+      - cbn in Hzzlen; lia.
+      - lia.
+      - rewrite app_length /=; lia.
+    }
+    { iIntros "!> !> %z %Hz0 %Hzlen (Hbuf&Hℓ)".
+      assert (exists zvres, zz !! (Z.to_nat z) = Some zvres) as [zvres Heq].
+      1: apply lookup_lt_is_Some_2; lia.
+      wp_pures. wp_apply (wp_loadN with "Hℓ"). 1: lia.
+      1: change (map ?f zz) with (fmap f zz); rewrite list_lookup_fmap Heq /= //.
+      iIntros "Hℓ". iExists _.
+      iSplit; first done. iFrame.
+      iExists (Z.to_nat z). iSplit; first (iPureIntro; lia).
+      done.
+    }
+    { by iIntros "($&$)". }
+    iIntros "!> (Hinbuf&Hℓ)". wp_finish.
+    wp_pures.
+
+    iPoseProof (isBufferRecordML_ext _ _ _ (λ z b, ⌜z = length zz⌝ ∗ ⌜b = map Some zz⌝)%I with "[] Hinbuf") as "Hinbuf".
+    { iIntros (z lst) "(%zpre&%zopost&%zzpost&->&%Hlenpost&->&%HH&%Hlenpre)".
+      assert (z = length (zpre ++ zzpost)) as -> by lia. iSplit; first done.
+      rewrite app_length in Hlenpre. assert (length zzpost = 0) as Hlen0 by lia.
+      destruct zzpost; last done. destruct zopost; last done.
+      by rewrite !app_nil_r. }
+
+    wp_extern. iModIntro. iLeft. iRight.
+    iExists _, _, _, _, zz, nil, (λ _ _, True)%I. do 3 iExists _. unfold named.
+    iSplit; first done.
+    iSplit; first done.
+    iFrame "Houtbuf". iSplit; first (cbn; iPureIntro; lia).
+    iSplitL "Hinbuf".
+    { iApply (isBufferRecordML_ext with "[] Hinbuf").
+      iIntros (z lst) "(->&->)". rewrite app_nil_r. done. }
+    iIntros "!> Hinbuf Houtbuf".
+    wp_pures.
+
+    iNamed "Hinbuf".
+    iDestruct "Houtbuf" as "(%ℓMLout&%used2&%fid2&%γfgn2&->&HℓbufMLout&Hbuf2)".
+    unfold named. wp_pures.
+    wp_apply (wp_load with "HℓbufML").
+    iIntros "HℓbufML". wp_pures.
+    wp_apply (wp_load with "HℓbufMLout").
+    iIntros "HℓbufMLout". wp_pures.
+    iAssert (⌜used = length zz⌝)%I as "->".
+    { iNamed "Hbuf". unfold named. iDestruct "HContent" as "(_&%&_)"; done. }
+    iAssert (⌜used2 = length (compress_buffer zz)⌝)%I as "->".
+    { iNamed "Hbuf2". unfold named. iDestruct "HContent" as "(%&%&%&_&%&_)"; done. }
+
+    wp_extern. do 2 iLeft. iRight.
+    iModIntro. iExists _, _, (λ _ _, _)%I, _.
+    do 2 (iSplit; first done).
+    iSplitL "Hbuf HℓbufML".
+    { do 4 iExists _. iSplit; first done. iFrame. }
+    iIntros "!> % % % _ _ _ _". wp_pures.
+
+    wp_extern. do 2 iLeft. iRight.
+    iModIntro. iExists _, _, (λ _ _, _)%I, _.
+    do 2 (iSplit; first done).
+    iSplitL "Hbuf2 HℓbufMLout".
+    { do 4 iExists _. iSplit; first done. iFrame. }
+    iIntros "!> % % % _ _ _ _". wp_pures.
+    unfold is_compressible. rewrite bool_decide_decide.
+    repeat destruct decide; cbn in *; try lia.
+    all: iApply ("Cont" with "Hℓ").
+  Qed.
+
+  Definition ML_client_applied_code : expr := if: ML_client_code (AllocN #256 #0) then #1 else #0.
+  Lemma ML_client_applied_spec :
+    {{{ True }}}
+      ML_client_applied_code @ ML_client_env ; E
+    {{{ x, RET #x ; ⌜x=1%Z⌝ }}}.
+  Proof.
+    iIntros (Φ) "_ Cont".
+    unfold ML_client_applied_code.
+    wp_apply (wp_allocN); [done..|].
+    iIntros (ℓ) "(Hℓ&_)".
+    wp_apply (ML_client_spec _ _ (replicate 256 (0:Z)) with "Hℓ"). 1: rewrite replicate_length; lia.
+    iIntros "_". wp_pures. by iApply "Cont".
+  Qed.
+
+End MLclient.
