theories/examples/compression/buffers_laws.v
@@ -1,0 +1,125 @@
+From iris.proofmode Require Import coq_tactics reduction spec_patterns.
+From iris.proofmode Require Export tactics.
+From iris.prelude Require Import options.
+From melocoton Require Import named_props.
+From melocoton.interop Require Import basics basics_resources basics_constructions.
+From melocoton.interop Require Import lang update_laws weakestpre.
+From melocoton.language Require Import weakestpre progenv.
+From melocoton.ml_lang Require Import notation lang_instantiation.
+From melocoton.ml_lang Require primitive_laws proofmode.
+From melocoton.c_interface Require Import defs notation resources.
+From melocoton.examples.compression Require Import buffers_specs.
+
+
+Section Specs.
+
+  Context `{SI:indexT}.
+  Context `{!heapG_C Σ, !heapG_ML Σ, !invG Σ, !primitive_laws.heapG_ML Σ, !wrapperG Σ}.
+
+  Lemma bufToML lv ℓbuf Pb c θ:
+      GC θ
+   -∗ isBufferRecord lv ℓbuf Pb c
+  ==∗ GC θ ∗ ∃ v, isBufferRecordML v ℓbuf Pb c ∗ lv ~~ v.
+  Proof.
+    iIntros "HGC H". iNamed "H". iNamed "Hbuf".
+    iMod (mut_to_ml _ ([ML_lang.LitV used]) with "[$HGC $Hγusedref]") as "(HGC&(%ℓML&HℓbufML&#HγML))".
+    1: by cbn.
+    iModIntro. iFrame "HGC".
+    iExists _. iSplitL.
+    { iExists ℓML, _, fid, γfgn. unfold named.
+      iSplit; first done. iFrame "HℓbufML".
+      iExists vcontent.
+      unfold named. by iFrame "Hγfgnpto Hℓbuf Hγfgnsim HContent". }
+    { cbn. iExists _, _, _. iSplitL; first done.
+      iFrame "Hγbuf".
+      iSplitL; first (iExists _; iSplit; done).
+      iExists _, _, _. iSplit; first done.
+      iFrame "Hγaux". iSplit; first done.
+      iExists _; iSplit; done. }
+  Qed.
+
+  Lemma bufToC v ℓbuf Pb c lv θ:
+      GC θ
+   -∗ isBufferRecordML v ℓbuf Pb c
+   -∗ lv ~~ v
+  ==∗ GC θ ∗ isBufferRecord lv ℓbuf Pb c ∗ ∃ (ℓML:loc) fid, ⌜v = (ML_lang.LitV ℓML, (ML_lang.LitV c, ML_lang.LitV (LitForeign fid)))%MLV⌝.
+  Proof.
+    iIntros "HGC H Hsim". iNamed "H". iNamed "Hbuf".
+    iDestruct "Hsim" as "#(%γ&%&%&->&Hγbuf&(%γref&->&Hsim)&%γaux&%&%&->&Hγaux&->&%γfgn2&->&Hγfgnsim2)".
+    iPoseProof (lloc_own_foreign_inj with "Hγfgnsim2 Hγfgnsim [$]") as "(HGC&%Hiff)".
+    destruct Hiff as [_ ->]; last done.
+    iMod (ml_to_mut with "[$HGC $HℓbufML]") as "(HGC&(%ℓvs&%γref2&Hγusedref&#Hsim2&#Hγrefsim))".
+    iPoseProof (lloc_own_pub_inj with "Hsim2 Hsim [$]") as "(HGC&%Hiff)".
+    destruct Hiff as [_ ->]; last done.
+    iModIntro. iFrame "HGC". iSplit; last by repeat iExists _. 
+    iExists _, _, _, _, _, _. unfold named.
+    iSplit; first done.
+    iFrame "Hγbuf". iFrame "Hγaux".
+    iSplitL "Hγusedref".
+    { destruct ℓvs as [|ℓvs [|??]]; cbn; try done.
+      all: iDestruct "Hγrefsim" as "[-> ?]"; try done. }
+    { cbn. iExists _. unfold named. iFrame "Hγfgnpto Hγfgnsim Hℓbuf HContent".
+      iPureIntro; done. }
+  Qed.
+
+  Lemma bufToC_fixed ℓbuf Pb (c:nat) ℓML fid lv θ:
+      GC θ
+   -∗ isBufferRecordML (ML_lang.LitV ℓML, (ML_lang.LitV c, ML_lang.LitV (LitForeign fid))) ℓbuf Pb c
+   -∗ lv ~~ (ML_lang.LitV ℓML, (ML_lang.LitV c, ML_lang.LitV (LitForeign fid)))
+  ==∗ GC θ ∗ isBufferRecord lv ℓbuf Pb c.
+  Proof.
+    iIntros "HGC H #Hsim".
+    iMod (bufToC with "HGC H Hsim") as "($&$&%ℓML1&%fid1&%Href)". done.
+  Qed.
+
+  Lemma bufToML_fixed lv ℓbuf Pb c (ℓML:loc) fid θ:
+      GC θ
+   -∗ isBufferRecord lv ℓbuf Pb c
+   -∗ lv ~~ (ML_lang.LitV ℓML, (ML_lang.LitV c, ML_lang.LitV (LitForeign fid)))
+  ==∗ GC θ ∗ isBufferRecordML (ML_lang.LitV ℓML, (ML_lang.LitV c, ML_lang.LitV (LitForeign fid))) ℓbuf Pb c.
+  Proof.
+    iIntros "HGC H #Hsim".
+    iMod (bufToML with "HGC H") as "(HGC&%&HML&#Hsim2)".
+    iAssert (⌜v = (ML_lang.LitV ℓML, (ML_lang.LitV c, ML_lang.LitV (LitForeign fid)))%MLV⌝)%I as "->"; last by iFrame.
+    iNamed "HML".
+    cbn.
+    iDestruct "Hsim" as "#(%γ&%&%&->&Hγbuf&(%γref&->&Hsim)&%γaux&%&%&->&Hγaux&->&%γfgn2&->&Hγfgnsim2)".
+    iDestruct "Hsim2" as "#(%γ2&%&%&%HHH&Hγbuf2&(%γref2&->&Hsim2)&%γaux2&%&%&->&Hγaux2&->&%γfgn3&->&Hγfgnsim3)".
+    simplify_eq.
+    unfold lstore_own_vblock, lstore_own_elem; cbn.
+    iDestruct "Hγbuf" as "(Hγbuf&_)".
+    iDestruct "Hγbuf2" as "(Hγbuf2&_)".
+    iDestruct "Hγaux" as "(Hγaux&_)".
+    iDestruct "Hγaux2" as "(Hγaux2&_)".
+    iPoseProof (ghost_map.ghost_map_elem_agree with "Hγbuf Hγbuf2") as "%Heq1"; simplify_eq.
+    iPoseProof (ghost_map.ghost_map_elem_agree with "Hγaux Hγaux2") as "%Heq1"; simplify_eq.
+    iPoseProof (lloc_own_foreign_inj with "Hγfgnsim2 Hγfgnsim3 HGC") as "(HGC&%Heq1)"; simplify_eq.
+    iPoseProof (lloc_own_pub_inj with "Hsim Hsim2 HGC") as "(HGC&%Heq2)"; simplify_eq.
+    iPureIntro. f_equal; repeat f_equal.
+    - symmetry; by eapply Heq2.
+    - symmetry; by eapply Heq1.
+  Qed.
+
+End Specs.
+
+Section LemmasThatShouldBeInStdPP.
+
+  Lemma map_replicate {A B : Type} (f : A → B) (v:A) n : map f (replicate n v) = replicate n (f v).
+  Proof.
+    induction n as [|n IH]; cbn; firstorder congruence.
+  Qed.
+
+  Lemma map_insert {A B : Type} (vpre : A) (f : A → B) (k : nat) (v : B) lst :
+    v = f vpre →
+    k < length lst →
+    <[ k := v ]> (map f lst) = map f (<[ k := vpre ]> lst).
+  Proof.
+    intros Hv.
+    induction lst as [|lh lr IH] in k|-*.
+    1: cbn; lia.
+    destruct k as [|k].
+    - intros _. cbn. by subst v.
+    - cbn. intros H%Nat.succ_lt_mono. by rewrite IH.
+  Qed.
+
+End LemmasThatShouldBeInStdPP.
