theories/examples/compression/buffers_proof_free.v
@@ -1,0 +1,93 @@
+From iris.proofmode Require Import coq_tactics reduction spec_patterns.
+From iris.proofmode Require Export tactics.
+From iris.prelude Require Import options.
+From melocoton Require Import named_props.
+From melocoton.interop Require Import basics basics_resources basics_constructions.
+From melocoton.interop Require Import lang weakestpre update_laws prims_proto.
+From melocoton.language Require Import weakestpre progenv.
+From melocoton.c_interop Require Import rules notation.
+From melocoton.ml_lang Require Import notation lang_instantiation.
+From melocoton.c_lang Require Import lang_instantiation.
+From melocoton.ml_lang Require primitive_laws proofmode.
+From melocoton.c_lang Require Import notation proofmode derived_laws.
+From melocoton.examples.compression Require Import buffers_specs buffers_laws buffers_code.
+
+Section Proofs.
+
+  Context `{SI:indexT}.
+  Context `{!heapG_C Σ, !heapG_ML Σ, !invG Σ, !primitive_laws.heapG_ML Σ, !wrapperG Σ}.
+
+
+  Lemma buf_free_correct E Ψ :
+    prims_proto E Ψ ||- buf_lib_prog @ E :: wrap_proto (buf_free_spec_ML).
+  Proof.
+    iIntros (s ws Φ) "H". iNamed "H".
+    iNamed "Hproto".
+    cbn. unfold progwp. solve_lookup_fixed.
+    destruct lvs as [|lv [|??]]; first done.
+    all: cbn; iDestruct "Hsim" as "(Hsim&H)"; try done.
+    destruct ws as [|w [|??]]; try (eapply Forall2_length in Hrepr; cbn in Hrepr; done).
+    eapply Forall2_cons_inv_l in Hrepr as (wγ&?&Hlγ&_&?); simplify_eq.
+    cbn. iExists _. iSplit; first done.
+    iExists _. cbn. solve_lookup_fixed.
+    iSplit; first done. iNext.
+
+    iMod (bufToC with "HGC Hbuf Hsim") as "(HGC&HBuf1&%&%&->)".
+    iNamed "HBuf1". iNamed "Hbuf".
+    wp_apply (wp_readfield with "[$HGC $Hγbuf]"); [done..|].
+    iIntros (vγaux1 wγaux1) "(HGC&_&%Heq1&%Hreprγaux1)". cbv in Heq1; simplify_eq.
+    wp_apply (wp_readfield with "[$HGC $Hγaux]"); [done..|].
+    iIntros (vγfgn1 wγfgn1) "(HGC&_&%Heq1&%Hreprγfgn1)". cbv in Heq1; simplify_eq.
+    wp_apply (wp_read_foreign with "[$HGC $Hγfgnpto]"); [done..|].
+    iIntros "(HGC&Hγfgnpto)". wp_pure _.
+
+    wp_apply (wp_readfield with "[$HGC $Hγbuf]"); [done..|].
+    iIntros (vγref1 wγref1) "(HGC&_&%Heq1&%Hreprγref1)". cbv in Heq1; simplify_eq.
+    wp_apply (wp_readfield with "[$HGC $Hγaux]"); [done..|].
+    iIntros (vv wcap) "(HGC&_&%Heq1&%Hreprwcap)". change (Z.to_nat 0) with 0 in Heq1; cbn in Heq1; simplify_eq.
+    wp_apply (wp_val2int with "HGC"); [done..|].
+    iIntros "HGC". wp_pure _.
+    wp_pure _; first by destruct ℓ. do 2 wp_pure _.
+    replace (length vcontent) with 
+      (length (map (option_map (λ z : Z, #z)) vcontent)) by by rewrite map_length.
+    wp_apply (wp_free_array with "Hℓbuf"). iIntros "_".
+    wp_pure _.
+
+    wp_apply (wp_readfield with "[$HGC $Hγbuf]"); [done..|].
+    iIntros (vγaux2 wγaux2) "(HGC&_&%Heq1&%Hreprγaux2)". cbv in Heq1; simplify_eq.
+    wp_apply (wp_readfield with "[$HGC $Hγaux]"); [done..|].
+    iIntros (vγfgn2 wγfgn2) "(HGC&_&%Heq1&%Hreprγfgn2)". cbv in Heq1; simplify_eq.
+    wp_apply (wp_write_foreign with "[$HGC $Hγfgnpto]"); [done..|].
+    iIntros "(HGC&Hγfgnpto)". wp_pure _.
+
+    wp_apply (wp_readfield with "[$HGC $Hγbuf]"); [done..|].
+    iIntros (vγref2 wγref2) "(HGC&_&%Heq1&%Hreprγref2)". cbv in Heq1; simplify_eq.
+    wp_apply (wp_int2val with "HGC"); [done..|].
+    iIntros (wnum) "(HGC&%Hreprm1)".
+    wp_apply (wp_modify with "[$HGC $Hγusedref]"); [done..|].
+    change (Z.to_nat 0) with 0. cbn.
+    iIntros "(HGC&Hγusedref)". wp_pure _.
+    iApply (wp_post_mono with "[HGC]").
+    1: wp_apply (wp_int2val with "HGC"); [done..|iIntros (w) "?"; iAccu].
+    iIntros (w) "(HGC&%Hwunit)".
+    iMod (mut_to_ml _ [ ML_lang.LitV (-1)%Z ] _ with "[$HGC $Hγusedref]") as "(HGC&%ℓML'&Hγusedref&#Hsim')". 1: cbn; iFrame; done.
+
+    iAssert (⌜ℓML' = ℓML⌝ ∗ ⌜fid0 = fid⌝)%I as "(->&->)".
+    { iDestruct "Hsim" as "#(%γ2&%&%&%HHH&Hγbuf2&(%γref2&->&Hsim2)&%γaux2&%&%&->&Hγaux2&->&%γfgn3&->&Hγfgnsim3)".
+      simplify_eq.
+      unfold lstore_own_vblock, lstore_own_elem; cbn.
+      iDestruct "Hγbuf" as "(Hγbuf&_)".
+      iDestruct "Hγbuf2" as "(Hγbuf2&_)".
+      iDestruct "Hγaux" as "(Hγaux&_)".
+      iDestruct "Hγaux2" as "(Hγaux2&_)".
+      iPoseProof (ghost_map.ghost_map_elem_agree with "Hγbuf Hγbuf2") as "%Heq1"; simplify_eq.
+      iPoseProof (ghost_map.ghost_map_elem_agree with "Hγaux Hγaux2") as "%Heq1"; simplify_eq.
+      iPoseProof (lloc_own_foreign_inj with "Hγfgnsim Hγfgnsim3 HGC") as "(HGC&%Heq1)"; simplify_eq.
+      iPoseProof (lloc_own_pub_inj with "Hsim' Hsim2 HGC") as "(HGC&%Heq2)"; simplify_eq.
+      iSplit; iPureIntro; [eapply Heq2|eapply Heq1]; done.
+    }
+    iModIntro.
+    iApply ("Cont" $! _  (ML_lang.LitV ())%MLV with "HGC (HCont [//] Hγfgnsim Hγusedref Hγfgnpto) [//] [//]").
+  Qed.
+
+End Proofs.
