theories/examples/compression/buffers_proof_update.v
@@ -1,0 +1,202 @@
+From iris.proofmode Require Import coq_tactics reduction spec_patterns.
+From iris.proofmode Require Export tactics.
+From iris.prelude Require Import options.
+From melocoton Require Import named_props.
+From melocoton.interop Require Import basics basics_resources basics_constructions.
+From melocoton.interop Require Import lang weakestpre update_laws prims_proto.
+From melocoton.language Require Import weakestpre progenv.
+From melocoton.c_interop Require Import rules notation.
+From melocoton.ml_lang Require Import notation lang_instantiation.
+From melocoton.c_lang Require Import lang_instantiation.
+From melocoton.ml_lang Require primitive_laws proofmode.
+From melocoton.c_lang Require Import notation proofmode derived_laws.
+From melocoton.examples.compression Require Import buffers_specs buffers_code buffers_laws.
+
+Section Proofs.
+
+  Context `{SI:indexT}.
+  Context `{!heapG_C Σ, !heapG_ML Σ, !invG Σ, !primitive_laws.heapG_ML Σ, !wrapperG Σ}.
+
+  Lemma buf_upd_correct E Ψcb :
+    prims_proto E Ψcb ||- buf_lib_prog @ E :: wrap_proto (buf_update_spec_ML Ψcb E).
+  Proof.
+    iIntros (s ws Φ) "H". iNamed "H". iNamed "Hproto".
+    cbn. unfold progwp. solve_lookup_fixed.
+    destruct lvs as [|lvi [|lvj [| lvF [| lvbuf [|??]]]]]; try done.
+    all: cbn; iDestruct "Hsim" as "(->&Hsim)"; try done.
+    all: cbn; iDestruct "Hsim" as "(->&Hsim)"; try done.
+    all: cbn; iDestruct "Hsim" as "((%γF&->&HγF)&Hsim)"; try done.
+    all: cbn; iDestruct "Hsim" as "(Hsim&?)"; try done.
+    destruct ws as [|wi [|wj [|wF [|wbuf [|??]]]]]; try (eapply Forall2_length in Hrepr; cbn in Hrepr; done).
+    eapply Forall2_cons in Hrepr as (Hrepri&Hrepr).
+    eapply Forall2_cons in Hrepr as (Hreprj&Hrepr).
+    eapply Forall2_cons in Hrepr as (HreprF&Hrepr).
+    eapply Forall2_cons in Hrepr as (Hreprbuf&_).
+    cbn. iExists _. iSplit; first done.
+    iExists _. cbn. solve_lookup_fixed.
+    iSplit; first done. iNext.
+    wp_apply (wp_CAMLlocal with "HGC"); [done..|].
+    iIntros (ℓF) "(HGC&HℓF)"; wp_pures.
+    wp_apply (store_to_root with "[$HGC $HℓF]"); [done..|].
+    iIntros "(HGC&HℓF)". wp_pures.
+    wp_apply (wp_CAMLlocal with "HGC"); [done..|].
+    iIntros (ℓbf) "(HGC&Hℓbf)"; wp_pures.
+    wp_apply (store_to_root with "[$HGC $Hℓbf]"); [done..|].
+    iIntros "(HGC&Hℓbf)". wp_pure _.
+    iMod (bufToC with "HGC Hrecord Hsim") as "(HGC&Hrecord&%&%&->)".
+    iNamed "Hrecord". iNamed "Hbuf".
+
+    wp_apply (load_from_root with "[$HGC $Hℓbf]"); [done..|].
+    iIntros (wγ1) "(Hℓbf&HGC&%Hwγ1)".
+    wp_apply (wp_readfield with "[$HGC $Hγbuf]"); [done..|].
+    iIntros (? wγaux1) "(HGC&_&%Heq&%Hγaux'1)"; cbv in Heq; simplify_eq.
+    wp_apply (wp_readfield with "[$HGC $Hγaux]"); [done..|].
+    iIntros (? wγfgn1) "(HGC&_&%Heq&%Hγfgn'1)"; cbv in Heq; simplify_eq.
+    wp_apply (wp_read_foreign with "[$HGC $Hγfgnpto]"); [done..|].
+    iIntros "(HGC&Hγfgnpto)". wp_pure _.
+    wp_apply (wp_val2int with "HGC"); [done..|].
+    iIntros "HGC". wp_pure _.
+    wp_apply (wp_Malloc); [done..|].
+    change (Z.to_nat 1) with 1; cbn.
+    iIntros (ℓi) "((Hℓi&_)&_)". rewrite !loc_add_0. wp_pure _.
+    wp_apply (wp_val2int with "HGC"); [done..|].
+    iIntros "HGC".
+    wp_apply (wp_store with "Hℓi").
+    iIntros "Hℓi". wp_pure _.
+
+    iMod (bufToML_fixed (Lloc γ) ℓbuf (Pb i) (length vcontent)
+         with "HGC [Hγusedref Hℓbuf HContent Hγfgnpto] Hsim") as "(HGC&HBufML)".
+    { iExists _, _, _, _, _, _. unfold named. iSplit; first done.
+      iFrame "Hγusedref Hγbuf Hγaux".
+      iExists _. unfold named. by iFrame "Hγfgnpto Hγfgnsim Hℓbuf HContent". }
+    iMod ("HMergeInitial" with "[$Hframe $HBufML]") as "HΨ".
+    wp_bind (While _ _).
+
+    repeat match goal with [H : repr_lval _ _ ?x |- _] => clear H; try clear x end.
+
+    iRevert (Hb1 Hb2); iIntros "#Hb1 #Hb2".
+    revert Hb3.
+    generalize (length vcontent) as vcontent_length. intros vcontent_length Hb3.
+    clear vcontent.
+
+    wp_apply (wp_wand _ _ _ (λ _, ∃ θ, ℓF ↦roots Lloc γF ∗ ℓbf ↦roots Lloc γ ∗ GC θ ∗ Ψ (j + 1)%Z ∗ ℓi ↦C{DfracOwn 1} #(j + 1))%I
+              with "[HℓF Hℓbf Hℓi HGC HΨ]").
+    { iRevert "HMerge HWP Hb1 Hb2". iLöb as "IH" forall (i θ).
+      iIntros "#HMerge #HWP %Hb1 %Hb2".
+      wp_pure _.
+      wp_apply (wp_load with "Hℓi").
+      iIntros "Hℓi". wp_pure _.
+      rewrite bool_decide_decide. destruct decide; last first.
+      { wp_pures. iModIntro.
+        assert (i=j+1)%Z as -> by lia. iExists _. iFrame. }
+      wp_pure _.
+
+      wp_apply (wp_load with "Hℓi").
+      iIntros "Hℓi". wp_pures.
+      wp_apply (load_from_root with "[$HGC $HℓF]").
+      iIntros (wγF) "(HℓF&HGC&%HwγF)".
+      wp_apply (wp_load with "Hℓi").
+      iIntros "Hℓi".
+      wp_apply (wp_int2val with "HGC"); [done..|].
+      iIntros (wi) "(HGC&%Hwi)".
+      wp_apply (wp_callback _ _ _ _ _ _ _ _ _ _ _ _ (ML_lang.LitV i) with "[$HGC $HγF HΨ]"); [done..| |].
+      { cbn. iSplit; first done.
+        iNext. by iApply ("HWP" with "[] [] HΨ"). } cbn.
+      cbn.
+      iIntros (θ' vret lvret wret) "(HGC&(%zret&->&HΦz&HΨframe&HBuffer)&->&%Hzrep)".
+      wp_apply (wp_val2int with "HGC"); [done..|].
+      iIntros "HGC". iRename "Hγfgnsim" into "Hγfgnsim2". clear used.
+      iDestruct "HBuffer" as "(%ℓML0&%&%&%&%Heq&HℓbufML&Hbuf)". simplify_eq. unfold named.
+      iNamed "Hbuf".
+      assert (∃ (ni:nat), Z.of_nat ni = i) as (ni&<-) by (exists (Z.to_nat i); lia).
+      wp_apply (wp_store_offset with "Hℓbuf").
+      1: rewrite map_length; lia.
+      iIntros "Hℓbuf". erewrite (map_insert (Some zret)); [|done|lia].
+
+      wp_pure _.
+      wp_apply (load_from_root with "[$HGC $Hℓbf]"); [done..|].
+      iIntros (wbf1) "(Hℓbf&HGC&%Hwbf1)".
+      wp_apply (wp_readfield with "[$HGC $Hγbuf]"); [done..|].
+      iIntros (vγref wγref) "(HGC&_&%Heq&%Hvwγref)". cbv in Heq. simplify_eq.
+
+      iMod (ml_to_mut with "[$HGC $HℓbufML]") as "(HGC&%&%&HℓbufML&#Hsim2&HHsim2)".
+      destruct lvs as [|? [|??]].
+      1: cbn; done.
+      all: iDestruct "HHsim2" as "(->&HHr)"; try done. iClear "HHr".
+
+      iAssert (⌜fid1 = fid0⌝ ∗ ⌜γfgn0 = γfgn⌝ ∗ ⌜γ0 = γref⌝)%I as "(->&->&->)".
+      { iDestruct "Hsim" as "#(%γ2&%&%&%HHH&Hγbuf2&(%γref2&->&Hsim3)&%γaux2&%&%&->&Hγaux2&->&%γfgn3&->&Hγfgnsim3)".
+        simplify_eq.
+        unfold lstore_own_vblock, lstore_own_elem; cbn.
+        iDestruct "Hγbuf" as "(Hγbuf&_)".
+        iDestruct "Hγbuf2" as "(Hγbuf2&_)".
+        iDestruct "Hγaux" as "(Hγaux&_)".
+        iDestruct "Hγaux2" as "(Hγaux2&_)".
+        iPoseProof (ghost_map.ghost_map_elem_agree with "Hγbuf Hγbuf2") as "%Heq1"; simplify_eq.
+        iPoseProof (ghost_map.ghost_map_elem_agree with "Hγaux Hγaux2") as "%Heq1"; simplify_eq.
+        iPoseProof (lloc_own_foreign_inj with "Hγfgnsim2 Hγfgnsim3 HGC") as "(HGC&%Heq1)"; simplify_eq.
+        iPoseProof (lloc_own_foreign_inj with "Hγfgnsim Hγfgnsim3 HGC") as "(HGC&%Heq1b)"; simplify_eq.
+        iPoseProof (lloc_own_pub_inj with "Hsim3 Hsim2 HGC") as "(HGC&%Heq2)"; simplify_eq.
+        iPureIntro. split_and!. 1: symmetry; by eapply Heq1.
+        1: by eapply Heq1b. 1: symmetry; by eapply Heq2. }
+
+      wp_apply (wp_readfield with "[$HGC $HℓbufML]"); [done..|].
+      iIntros (vγbuf wγbuf) "(HGC&HℓbufML&%Heq&%Hvwγbuf)". change (Z.to_nat 0) with 0 in Heq. cbn in Heq. simplify_eq.
+      wp_apply (wp_val2int with "HGC"); [done..|].
+      iIntros "HGC".
+      wp_apply (wp_load with "Hℓi").
+      iIntros "Hℓi". do 2 wp_pure _.
+      wp_bind (If _ _ _).
+      iApply (wp_wand _ _ _ (λ _, _ ∗ γref ↦mut (TagDefault, [Lint (max used (Z.to_nat (ni+1)))%Z]))%I with "[HGC Hℓi Hℓbf HℓbufML]").
+      { rewrite bool_decide_decide. destruct decide; last first.
+        { do 2 wp_pure _. rewrite max_l; last lia.
+          iFrame "HℓbufML". iModIntro. iAccu. }
+        { wp_pure _.
+          wp_apply (load_from_root with "[$HGC $Hℓbf]"); [done..|].
+          iIntros (wbf2) "(Hℓbf&HGC&%Hwbf2)".
+          wp_apply (wp_readfield with "[$HGC $Hγbuf]"); [done..|].
+          iIntros (vγref2 wγref2) "(HGC&_&%Heq&%Hvwγref2)". cbv in Heq. simplify_eq.
+          wp_apply (wp_load with "Hℓi").
+          iIntros "Hℓi". wp_pure _.
+          wp_apply (wp_int2val with "HGC"); [done..|].
+          iIntros (vnp1) "(HGC&%Hnp1)".
+          wp_apply (wp_modify with "[$HGC $HℓbufML]"); [done..|].
+          iIntros "(HGC&HℓbufML)". iFrame "HGC Hℓbf Hℓi".
+          rewrite max_r; last lia. change (Z.to_nat 0) with 0; cbn.
+          rewrite Z2Nat.id; last lia. done. }
+      }
+      iIntros (vv) "((HGC&Hℓi&Hℓbf)&HℓbufML)". wp_pure _.
+      wp_apply (wp_load with "Hℓi"). iIntros "Hℓi". wp_pure _.
+      wp_apply (wp_store with "Hℓi"). iIntros "Hℓi". wp_pure _.
+      iMod (mut_to_ml _ [ ML_lang.LitV (_:Z)] with "[$HGC $HℓbufML]") as "(HGC&%ℓML2&HℓbufML&Hsimℓ2)". 1: cbn; iFrame; done.
+      iPoseProof (lloc_own_pub_inj with "Hsim2 Hsimℓ2 HGC") as "(HGC&%Heq3)"; simplify_eq.
+      replace ℓML2 with ℓML0 by by eapply Heq3.
+      iMod ("HMerge" with "[] [] HΨframe HΦz [Hγfgnpto HContent Hℓbuf HℓbufML]") as "HH". 1-2: iPureIntro; lia.
+      { iExists _, _, _, _. unfold named. iSplit; first done. iFrame "HℓbufML".
+        iExists _. unfold named. iFrame "Hγfgnpto Hγfgnsim Hℓbuf".
+        rewrite insert_length. iSplit; last done.
+        iExists vcontent, _. iFrame "HContent". iPureIntro. rewrite Nat2Z.id. split; first done.
+        reflexivity. }
+      iApply ("IH" with "HℓF Hℓbf Hℓi HGC HH").
+      - iIntros "!> %z1 %z2 %HH1 %HH2". iApply "HMerge".
+        all: iPureIntro; lia.
+      - iIntros "!> %z1 %HH1 %HH2". iApply "HWP".
+        all: iPureIntro; lia.
+      - iPureIntro; lia.
+      - iPureIntro; lia.
+    }
+    iIntros (vvv) "(%θ' & HℓF & Hℓbf & HGC & HΨ & Hℓi)".
+    wp_pure _.
+    wp_apply (wp_free with "Hℓi"). iIntros "_".
+    wp_pure _.
+    wp_apply (wp_int2val with "HGC"); [done..|].
+    iIntros (v0) "(HGC&%Hrepr)".
+    wp_pure _.
+    wp_apply (wp_CAMLunregister1 with "[$HGC $HℓF]"); [done..|].
+    iIntros "HGC"; wp_pure _.
+    wp_apply (wp_CAMLunregister1 with "[$HGC $Hℓbf]"); [done..|].
+    iIntros "HGC"; wp_pure _.
+    iModIntro. iApply ("Cont" with "HGC (HCont HΨ) [//] [//]").
+  Qed.
+
+End Proofs.
