theories/examples/compression/buffers_proofs.v
@@ -1,0 +1,63 @@
+From iris.proofmode Require Import coq_tactics reduction spec_patterns.
+From iris.proofmode Require Export tactics.
+From iris.prelude Require Import options.
+From melocoton Require Import named_props.
+From melocoton.interop Require Import basics basics_resources basics_constructions.
+From melocoton.interop Require Import lang weakestpre update_laws prims_proto.
+From melocoton.language Require Import weakestpre progenv wp_link.
+From melocoton.c_interop Require Import rules notation.
+From melocoton.ml_lang Require Import notation lang_instantiation.
+From melocoton.c_lang Require Import lang_instantiation.
+From melocoton.ml_lang Require primitive_laws proofmode.
+From melocoton.c_lang Require Import notation proofmode derived_laws.
+From melocoton.examples.compression Require Import buffers_specs buffers_laws buffers_code 
+  compression_specs compression_proofs
+  buffers_proof_alloc buffers_proof_update buffers_proof_free buffers_proofs_compr.
+
+
+Section Proofs.
+
+  Context `{SI:indexT}.
+  Context `{!heapG_C Σ, !heapG_ML Σ, !invG Σ, !primitive_laws.heapG_ML Σ, !wrapperG Σ}.
+
+  Definition buf_lib_prog_total : gmap _ _ := buf_lib_prog ∪ buffy_env.
+
+  Lemma buffer_library_correct_pre E Ψ :
+    (buffy_library_spec ⊔ prims_proto E Ψ) ||- buf_lib_prog @ E :: wrap_proto (buf_library_spec_ML_pre E Ψ).
+  Proof.
+    iIntros (s vv Φ) "H". iNamed "H".
+    iDestruct "Hproto" as "[[[[Hproto|Hproto]|Hproto]|Hproto]|Hproto]".
+    - iApply progwp_mono; [done|eapply prims_proto_refines_combspec|].
+      iApply buf_alloc_correct. do 4 iExists _. iFrameNamed.
+    - iApply progwp_mono; [done|eapply prims_proto_refines_combspec|].
+      iApply buf_upd_correct. do 4 iExists _. iFrameNamed.
+    - iApply progwp_mono; [done|eapply prims_proto_refines_combspec|].
+      iApply buf_free_correct. do 4 iExists _. iFrameNamed.
+    - iApply wrap_compress_correct. do 4 iExists _. iFrameNamed.
+    - iApply wrap_max_len_correct. do 4 iExists _. iFrameNamed.
+  Qed.
+
+  Lemma buffer_library_correct E Ψ :
+    prims_proto E Ψ ||- buf_lib_prog_total @ E :: wrap_proto (buf_library_spec_ML_pre E Ψ).
+  Proof.
+    eassert (can_link_all E (prims_proto E Ψ) (wrap_proto (buf_library_spec_ML_pre E Ψ)) buf_lib_prog_total _) as Hlink.
+    - eapply can_link_can_link_all.
+      assert (buf_lib_prog ##ₘ buffy_env) as Hdisj.
+      1: { apply map_disjoint_dom. rewrite /buffy_env /buf_lib_prog !dom_insert_L !dom_empty_L. set_solver. }
+      econstructor.
+      5: eapply buffer_library_correct_pre.
+      4: eapply buffy_library_correct; done.
+      1: by apply map_disjoint_dom.
+      1: iIntros (s vv Φ) "H"; by iRight.
+      1: { iIntros (s vv Φ) "H"; iNamed "H".
+           cbn. rewrite !dom_union_L !dom_insert_L !dom_empty_L.
+           destruct p; try (iNamed "H"; iPureIntro; set_solver). cbn. done. }
+      eapply map_eq_iff. intros s.
+      rewrite /buf_lib_prog_total map_union_comm. 2:done. rewrite lookup_union lookup_union_with.
+      destruct (buffy_env !! s) eqn:Heq1; rewrite Heq1;
+      destruct (buf_lib_prog !! s) eqn:Heq2; try done.
+      eapply map_disjoint_Some_l in Heq2; last done. rewrite Heq1 in Heq2. by congruence.
+    - apply (wp_link_progs _ _ _ _ _ Hlink).
+  Qed.
+
+End Proofs.
