theories/examples/compression/compression_defs.v
@@ -1,0 +1,87 @@
+From iris.proofmode Require Export tactics.
+From iris.prelude Require Import options.
+
+Section SemBuffers.
+(* Of course, snappy is more complicated than this ..*)
+Definition buffer := list Z.
+
+Fixpoint compress_buffer (b:buffer) : buffer := (match b with
+| 0 :: 0 :: xs => 0 :: compress_buffer xs
+| x :: xs => 1 :: x :: compress_buffer xs
+| nil => nil end)%Z.
+
+Definition buffer_max_len (n : nat) := 2 * n.
+
+Fixpoint decompress_buffer (b:buffer) : option buffer := (match b with
+| 0 :: xs => option_map (λ x, 0 :: 0 :: x) (decompress_buffer xs)
+| 1 :: 0 :: 1 :: 0 :: xs => None
+| 1 :: 0 :: 0 :: xs => None
+| 1 :: x :: xs => option_map (cons x) (decompress_buffer xs)
+| nil => Some nil
+| _ => None end)%Z.
+
+Lemma decompress_compress b : decompress_buffer (compress_buffer b) = Some b.
+Proof.
+  induction b using (induction_ltof1 _ (@length _)); unfold ltof in *.
+  destruct x as [|b1 [|b2 br]].
+  - done.
+  - cbn. by case_match.
+  - cbn. repeat (case_match; try done).
+    all: cbn; rewrite H; last (cbn; lia); try done.
+Qed.
+
+Lemma decompress_to_nil b : decompress_buffer b = Some nil → b = nil.
+Proof.
+  destruct b; try done; cbn.
+  repeat (cbn in *; unfold option_map in *; case_match; simplify_eq; try done).
+Qed.
+
+Lemma compress_decompress b b2 : decompress_buffer b = Some b2 → compress_buffer b2 = b.
+Proof. revert b2.
+  induction b using (induction_ltof1 _ (@length _)); unfold ltof in *; intros bb Hb.
+  destruct x as [|b1 br].
+  - cbn in *. by simplify_eq.
+  - repeat (cbn in *; case_match; simplify_eq; try done); unfold option_map in *.
+    + case_match; last done.
+      simplify_eq. eapply H in H0; last (cbn; lia). subst br; done.
+    + case_match; last done. simplify_eq. eapply H in H0; last (cbn; lia).
+      destruct b; first done. cbn in *; repeat (case_match; simplify_eq); done.
+    + destruct (decompress_buffer l) eqn:Heq; cbn in *; last done. simplify_eq.
+      eapply H in Heq; last (cbn; lia). subst l. cbn. done.
+    + destruct (decompress_buffer l) eqn:Heq; cbn in *; last done. simplify_eq.
+      eapply H in Heq; last (cbn; lia). subst l. cbn. done.
+    + case_match; last done. simplify_eq.
+      eapply H in H0; last (cbn; lia). subst l. cbn. done.
+    + case_match; last done. simplify_eq.
+      eapply H in H0; last (cbn; lia). subst l. cbn. done.
+Qed.
+
+Lemma max_len_correct b : length (compress_buffer b) ≤ buffer_max_len (length b).
+Proof.
+  induction b using (induction_ltof1 _ (@length _)); unfold ltof in *.
+  destruct x as [|b1 [|b2 br]].
+  - cbn in *; lia.
+  - cbn. by case_match.
+  - cbn. repeat (case_match; try (first [done | cbn in *; lia])).
+    all: cbn in *; repeat (first [eapply le_n_S | erewrite Nat.add_succ_r]); etransitivity; first eapply H; cbn in *; lia.
+Qed.
+
+Lemma max_len_tight n : ∃ b, length b = n ∧ length (compress_buffer b) = buffer_max_len n.
+Proof.
+  induction n as [|n (b&IH1&IH2)].
+  - exists []. done.
+  - exists (1 :: b)%Z. cbn; split_and!; try done; try lia.
+    rewrite IH2. unfold buffer_max_len. lia.
+Qed.
+
+Lemma compression_makes_shorter n : ∃ b, length b ≥ n ∧ length (compress_buffer b) < length b.
+Proof.
+  exists (repeat 0%Z (2*(S n))).
+  rewrite repeat_length. split; first lia.
+  induction n as [|n IH].
+  - cbn. lia.
+  - cbn. rewrite -!Nat.succ_lt_mono. cbn -[repeat] in IH. etransitivity.
+    1: erewrite Nat.add_succ_r; exact IH. lia.
+Qed.
+
+End SemBuffers.
